coq/def/Exprs.v
@@ -12,248 +12,15 @@ Require Import Ords.
 
 Set Implicit Arguments.
 
+Local Open Scope OrdIdx_scope.
 
-(* Module MSetAVLExtra (E: Orders.OrderedType). *)
-(*   (* Require Import MSets.MSetRBT. *) *)
-(*   (* MSetRBT.Make. *) *)
-(*   Include MSetAVL.Make E. *)
-(*   Definition notin x L := ~ In x L. *)
+(* TODO: Move to Ords.v *)
+Module Backport_Alt (E: OrdersAlt.OrderedTypeAlt) <: OrderedType.OrderedType.
+  Module OT := (OrdersAlt.OT_from_Alt E).
+  Include (OrdersAlt.Backport_OT OT).
+End Backport_Alt.
 
-(* End MSetAVLExtra. *)
-
-Module MSetAVLExtra (E: Orders.OrderedType).
-  (* Require Import MSets.MSetRBT. *)
-  (* MSetRBT.Make. *)
-  (* Module Mod_A : OrdersAlt.OrderedTypeAlt := Alt_from_AltUsual E. *)
-  (* Module Mod_OT := OrdersAlt.OT_from_Alt Mod_A. *)
-  (* Module Mod_OT := OrdersAlt.OT_from_Alt E. *)
-
-  Include MSetAVL.Make E.
-  Definition notin x L := ~ In x L.
-  Definition add_list (xs: list E.t) (base: t): t :=
-    List.fold_left (fun s i => add i s) xs base
-  .
-
-End MSetAVLExtra.
-
-Module MSetFactsExtra (E: Orders.OrderedType) (M: MSetInterface.S with Module E := E).
-
-(* Module MSetFactsExtra (E: Orders.OrderedType) (M: (MSetInterface.SetsOn E)). *)
-
-  Include MSetFacts.Facts M.
-
-  Definition map f s := M.fold (compose M.add f) s M.empty.
-
-  Lemma exists_false_iff
-        s f
-        (COMPAT: compat_bool E.eq f):
-    ~ M.Exists (fun x : M.elt => f x = true) s <->
-    M.exists_ f s = false.
-  Proof.
-    econs; ii.
-    - destruct (M.exists_ f s) eqn:X; ss.
-      contradict H. apply exists_iff; ss.
-    - apply exists_iff in H0; ss. clarify.
-  Qed.
-
-  Lemma exists_filter
-        pred1 pred2 ids
-        (PRED1: compat_bool E.eq pred1)
-        (PRED2: compat_bool E.eq pred2)
-    : M.exists_ pred1 (M.filter pred2 ids) =
-      M.exists_ (fun x => andb (pred1 x) (pred2 x)) ids.
-  Proof.
-    destruct (M.exists_ pred1 (M.filter pred2 ids)) eqn:X1.
-    - apply exists_iff in X1; [|solve_compat_bool].
-      inv X1. des. apply filter_iff in H; [|solve_compat_bool]. des.
-      symmetry. apply exists_iff; ss.
-      { ii. f_equal; eauto. }
-      econs. esplits; eauto. apply andb_true_iff. ss.
-    - symmetry. apply exists_false_iff.
-      { ii. f_equal; eauto. }
-      apply exists_false_iff in X1; ss. contradict X1.
-      inv X1. des. apply andb_true_iff in H0. des.
-      econs. splits; eauto. apply filter_iff; ss.
-  Qed.
-
-  Lemma map_spec f s ty
-        (F: Proper (E.eq ==> E.eq) f):
-    M.mem ty (map f s) =
-    M.exists_ (eqb ty <*> f) s.
-  Proof.
-    unfold map. rewrite M.fold_spec, <- fold_left_rev_right.
-    rewrite exists_b; cycle 1.
-    { ii. unfold eqb, compose.
-      destruct (eq_dec ty (f x)), (eq_dec ty (f y)); ss.
-      - contradict n. etransitivity; eauto.
-      - contradict n. etransitivity; eauto. eapply F; eauto. symmetry. ss.
-    }
-    rewrite existsb_rev.
-    induction (rev (M.elements s)); ss.
-    - destruct (M.mem ty M.empty) eqn:X; ss.
-      apply M.mem_spec in X. exfalso. eapply M.empty_spec. eauto.
-    - unfold compose, flip in *. rewrite add_b, IHl0.
-      f_equal. unfold eqb. destruct (eq_dec (f a) ty), (eq_dec ty (f a)); ss.
-      + contradict n. symmetry. ss.
-      + contradict n. symmetry. ss.
-  Qed.
-
-  Definition from_list
-             (ids:list E.t): M.t :=
-    fold_left (flip M.add) ids M.empty.
-
-  Lemma from_list_spec ids:
-    forall id, M.mem id (from_list ids) <-> InA E.eq id ids.
-  Proof.
-    unfold from_list. rewrite <- fold_left_rev_right.
-    intros. rewrite <- InA_rev.
-    unfold M.elt.
-    match goal with
-    | [|- context[@rev ?T ?ids]] => induction (@rev T ids)
-    end; simpl.
-    - rewrite empty_b. intuition. inv H.
-    - unfold flip in *. rewrite add_b.
-      unfold eqb. constructor; intros.
-      + apply orb_true_iff in H. destruct H.
-        * left. destruct (eq_dec a id0); intuition.
-        * right. apply IHl0. auto.
-      + apply orb_true_intro. inv H.
-        * destruct (eq_dec a id0); auto.
-          contradict n. symmetry. ss.
-        * right. apply IHl0. auto.
-  Qed.
-
-End MSetFactsExtra.
-
-
-(* Default OrderedType is Structures.OrderedType *)
-(* https://coq.inria.fr/library/ *)
-(* ... OrderedType* are there only for compatibility. *)
-
-Module Tag <: AltUsual.
-  Inductive t_: Set :=
-  | physical
-  | previous
-  | ghost
-  .
-  Definition t := t_.
-
-  Definition eq := @eq t.
-  Definition eq_refl := @refl_equal t.
-  Definition eq_sym := @sym_eq t.
-  Definition eq_trans := @trans_eq t.
-  Definition eq_dec (x y:t): {x = y} + {x <> y}.
-    decide equality.
-  Defined.
-  Global Program Instance eq_equiv : Equivalence eq.
-
-  Definition is_previous x := match x with Tag.previous => true | _ => false end.
-  Definition is_ghost x := match x with Tag.ghost => true | _ => false end.
-
-  (* physical < previous < ghost *)
-  Definition ltb (x y: t): bool :=
-    match x, y with
-    | physical, previous => true
-    | physical, ghost => true
-    | previous, ghost => true
-    | _, _ => false
-    end.
-
-  (* Definition lt: t -> t -> Prop := ltb. *)
-
-  Definition compare (x y: t): comparison :=
-    if(eq_dec x y) then Eq else
-      (if (ltb x y) then Lt else Gt)
-  .
-  
-  (* Lemma compare_spec : forall x y : t, CompareSpec (eq x y) (lt x y) (lt y x) (compare x y). *)
-  (* Proof. *)
-  (*   ii. destruct x, y; ss; by econs. *)
-  (* Qed. *)
-
-  (* Global Program Instance lt_strorder : StrictOrder lt. *)
-  (* Next Obligation. *)
-  (*   ii. unfold lt in *. unfold ltb in *. des_ifs. *)
-  (* Qed. *)
-
-  (* Global Program Instance lt_compat : Proper (eq ==> eq ==> iff) lt. *)
-  (* Next Obligation. *)
-  (*   ii. unfold eq in *. clarify. *)
-  (* Qed. *)
-  (* Next Obligation. *)
-  (*   ii. unfold lt in *. unfold ltb in *. des_ifs. *)
-  (* Qed. *)
-
-  Lemma compare_sym : forall x y : t, << SYM: compare y x = CompOpp (compare x y) >>.
-  Proof. destruct x, y; ss. Qed.
-
-  Lemma compare_trans :
-     forall (c : comparison) (x y z : t),
-       compare x y = c -> compare y z = c -> << TR:compare x z = c >>.
-  Proof. i. destruct x, y, z; ss; des_ifs. Qed.
-    
-  Lemma compare_leibniz : forall x y : t, compare x y = Eq -> x = y.
-  Proof. destruct x, y; ss. Qed.
-End Tag.
-
-
-
-(* Module Tag <: Orders.OrderedType. *)
-(*   Inductive t_: Set := *)
-(*   | physical *)
-(*   | previous *)
-(*   | ghost *)
-(*   . *)
-(*   Definition t := t_. *)
-(*   Definition eq := @eq t. *)
-(*   Definition eq_refl := @refl_equal t. *)
-(*   Definition eq_sym := @sym_eq t. *)
-(*   Definition eq_trans := @trans_eq t. *)
-(*   Definition eq_dec (x y:t): {x = y} + {x <> y}. *)
-(*     decide equality. *)
-(*   Defined. *)
-(*   Global Program Instance eq_equiv : Equivalence eq. *)
-
-(*   Definition is_previous x := match x with Tag.previous => true | _ => false end. *)
-(*   Definition is_ghost x := match x with Tag.ghost => true | _ => false end. *)
-
-(*   (* physical < previous < ghost *) *)
-(*   Definition ltb (x y: t): bool := *)
-(*     match x, y with *)
-(*     | physical, previous => true *)
-(*     | physical, ghost => true *)
-(*     | previous, ghost => true *)
-(*     | _, _ => false *)
-(*     end. *)
-
-(*   Definition lt: t -> t -> Prop := ltb. *)
-
-(*   Definition compare (x y: t): comparison := *)
-(*     if(eq_dec x y) then Eq else *)
-(*       (if (ltb x y) then Lt else Gt) *)
-(*   . *)
-  
-(*   Lemma compare_spec : forall x y : t, CompareSpec (eq x y) (lt x y) (lt y x) (compare x y). *)
-(*   Proof. *)
-(*     ii. destruct x, y; ss; by econs. *)
-(*   Qed. *)
-
-(*   Global Program Instance lt_strorder : StrictOrder lt. *)
-(*   Next Obligation. *)
-(*     ii. unfold lt in *. unfold ltb in *. des_ifs. *)
-(*   Qed. *)
-
-(*   Global Program Instance lt_compat : Proper (eq ==> eq ==> iff) lt. *)
-(*   Next Obligation. *)
-(*     ii. unfold eq in *. clarify. *)
-(*   Qed. *)
-(*   Next Obligation. *)
-(*     ii. unfold lt in *. unfold ltb in *. des_ifs. *)
-(*   Qed. *)
-
-(* End Tag. *)
-(* Hint Resolve Tag.eq_dec: EqDecDb. *)
-
+(* TODO: move to Ords.v *)
 Module prod (E1 E2: AltUsual) <: AltUsual.
 
   Definition t : Type := E1.t * E2.t.
@@ -334,48 +101,91 @@ Module prod (E1 E2: AltUsual) <: AltUsual.
 End prod.
 
 
+
+
+Module Tag <: AltUsual.
+  Inductive t_: Set :=
+  | physical
+  | previous
+  | ghost
+  .
+  Definition t := t_.
+  Definition eq := @eq t.
+  Definition eq_refl := @refl_equal t.
+  Definition eq_sym := @sym_eq t.
+  Definition eq_trans := @trans_eq t.
+  Definition eq_dec (x y:t): {x = y} + {x <> y}.
+    decide equality.
+  Defined.
+  Global Program Instance eq_equiv : Equivalence eq.
+
+  Definition is_previous x := match x with Tag.previous => true | _ => false end.
+  Definition is_ghost x := match x with Tag.ghost => true | _ => false end.
+
+  (* physical < previous < ghost *)
+  Definition ltb (x y: t): bool :=
+    match x, y with
+    | physical, previous => true
+    | physical, ghost => true
+    | previous, ghost => true
+    | _, _ => false
+    end.
+
+  (* Definition lt: t -> t -> Prop := ltb. *)
+
+  Definition compare (x y: t): comparison :=
+    if(eq_dec x y) then Eq else
+      (if (ltb x y) then Lt else Gt)
+  .
+
+  Lemma compare_sym : forall x y : t, << SYM: compare y x = CompOpp (compare x y) >>.
+  Proof. destruct x, y; ss. Qed.
+
+  Lemma compare_trans :
+     forall (c : comparison) (x y z : t),
+       compare x y = c -> compare y z = c -> << TR:compare x z = c >>.
+  Proof. i. destruct x, y, z; ss; des_ifs. Qed.
+
+  Lemma compare_leibniz : forall x y : t, compare x y = Eq -> x = y.
+  Proof. destruct x, y; ss. Qed.
+
+End Tag.
+
+Hint Resolve Tag.eq_dec: EqDecDb.
+
 Module IdT <: AltUsual.
   Include (prod Tag id).
 
+  Definition eq_dec (x y:t): {x = y} + {x <> y}.
+  Proof.
+    decide equality.
+    apply Tag.eq_dec.
+  Qed.
+
   Definition lift (tag:Tag.t) (i:id): t := (tag, i).
+
 End IdT.
-(* Module IdT_A := Alt_from_AltUsual IdT_AU. *)
-(* Module IdT <: Orders.OrderedType. *)
-(*    Include OT_from_AltUsual IdT_AU. *)
+Hint Resolve IdT.eq_dec: EqDecDb.
 
-(*    Definition lift (tag:Tag.t) (i:id): t := (tag, i). *)
+Module IdT_OT := Backport_Alt IdT.
 
-(* End IdT. *)
-Module IdTFacts := AltUsualFacts IdT.
-
-Hint Resolve IdTFacts.eq_dec_l: EqDecDb.
-(* Hint Resolve IdT.eql_dec: EqDecDb. *)
-
-
-(* Module IdTSet : FSetExtra.WSfun IdT := FSetExtra.Make IdT. *)
-(* Module IdTSetFacts := WFacts_fun2 IdT IdTSet. *)
-
-Print MSetInterface.
-Print MSetInterface.S.
-
-Module IdT_OT := OrdersAlt.OT_from_Alt IdT.
 Module IdTSet.
-  Include MSetAVLExtra IdT_OT.
+  Include FSetAVLExtra IdT_OT.
 
   Definition clear_idt (idt0: IdT.t) (t0: t): t :=
-    filter (fun x => negb (IdTFacts.eq_dec_l idt0 x)) t0
+    filter (fun x => negb (IdT.eq_dec idt0 x)) t0
   .
 
 End IdTSet.
 
-(* "MSetInterface.S with Module E := IdT" dosen't work *)
-Module IdTSetFacts := MSetFactsExtra IdT_OT IdTSet.
+Module IdTSetFacts := FSetFactsExtra IdT_OT IdTSet.
 
 Lemma IdTSet_from_list_spec ids:
   forall id, IdTSet.mem id (IdTSetFacts.from_list ids) <-> In id ids.
 Proof.
-(*   i. rewrite IdTSetFacts.from_list_spec. apply InA_iff_In. *)
-(* Qed. *)
+  i. rewrite IdTSetFacts.from_list_spec.
+  etransitivity; try apply InA_iff_In.
+  split; i.
 Admitted.
 
 Module Value.
@@ -388,15 +198,18 @@ Module Value.
     end.
 End Value.
 
-
-Local Open Scope OrdIdx_scope.
-
 Module ValueT <: AltUsual.
   Inductive t_: Type :=
   | id (x:IdT.t)
   | const (c:const)
   .
   Definition t:= t_.
+  Definition eq_dec (x y:t): {x = y} + {x <> y}.
+  Proof.
+    decide equality.
+    apply IdT.eq_dec.
+    apply const_dec.
+  Qed.
 
   Definition case_order v : OrdIdx.t :=
     match v with
@@ -446,140 +259,51 @@ Module ValueT <: AltUsual.
 
   Definition substitute (from: IdT.t) (to: ValueT.t) (body: ValueT.t): ValueT.t :=
     match body with
-    | id i => if(IdTFacts.eq_dec_l from i) then to else body
+    | ValueT.id i => if(IdT.eq_dec from i) then to else body
     | _ => body
     end
   .
 
-  
 End ValueT.
 
-Module ValueTFacts := AltUsualFacts ValueT.
-
-(* Module ValueT_A := Alt_from_AltUsual ValueT_AU. *)
-(* old *)
-
-
-(* Module ValueT <: Orders.OrderedType. *)
-
-(* Module ValueT <: UsualDecidableType. *)
-(*   Inductive t_: Set := *)
-(*   | id (x:IdT.t) *)
-(*   | const (c:const) *)
-(*   . *)
-(*   Definition t:= t_. *)
-(*   Definition eq := @eq t. *)
-(*   Definition eq_refl := @refl_equal t. *)
-(*   Definition eq_sym := @sym_eq t. *)
-(*   Definition eq_trans := @trans_eq t. *)
-(*   Definition eq_dec (x y:t): {x = y} + {x <> y}. *)
-(*   Proof. *)
-(*     decide equality. *)
-(*     apply IdT.eq_dec. *)
-(*     apply const_dec. *)
-(*   Qed. *)
-
-(*   Definition lift (tag:Tag.t) (v:value): t := *)
-(*     match v with *)
-(*     | value_id i => id (IdT.lift tag i) *)
-(*     | value_const c => const c *)
-(*     end. *)
-
-(*   Definition get_idTs (v: t): option IdT.t := *)
-(*     match v with *)
-(*       | id i => Some i *)
-(*       | const _ => None *)
-(*     end. *)
-
-(*   Definition substitute (from: IdT.t) (to: ValueT.t) (body: ValueT.t): ValueT.t := *)
-(*     match body with *)
-(*     | ValueT.id i => if(IdT.eq_dec from i) then to else body *)
-(*     | _ => body *)
-(*     end *)
-(*   . *)
-
-(* End ValueT. *)
-(* Hint Resolve ValueT.eq_dec: EqDecDb. *)
-Hint Resolve ValueTFacts.eq_dec_l: EqDecDb.
+Hint Resolve ValueT.eq_dec: EqDecDb.
 Coercion ValueT.id: IdT.t >-> ValueT.t_.
 Coercion ValueT.const: const >-> ValueT.t_.
 
-(* Module ValueTSet : FSetExtra.WSfun ValueT := FSetExtra.Make ValueT. *)
-(* Module ValueTSetFacts := WFacts_fun2 ValueT ValueTSet. *)
+Module ValueT_OT := Backport_Alt ValueT.
 
-Module ValueT_OT := OT_from_AltUsual ValueT.
+Module ValueTSet := FSetAVLExtra ValueT_OT.
+Module ValueTSetFacts := FSetFactsExtra ValueT_OT ValueTSet.
 
-Module ValueTSet.
-  Include MSetAVLExtra ValueT_OT.
-
-  (* Definition clear_idt (idt0: IdT.t) (t0: t): t := *)
-  (*   filter (fun x => negb (IdT.eq_dec idt0 x)) t0 *)
-  (* . *)
-
-End ValueTSet.
-
-(* "MSetInterface.S with Module E := IdT" dosen't work *)
-Module ValueTSetFacts := MSetFactsExtra ValueT_OT ValueTSet.
-
-Module ValueTPair.
+Module ValueTPair <: AltUsual.
   Include prod ValueT ValueT.
+
+  Definition eq_dec (x y:t): {x = y} + {x <> y}.
+  Proof.
+    apply prod_dec;
+    apply ValueT.eq_dec.
+  Defined.
 
   Definition get_idTs (vp: t): list IdT.t :=
     (option_to_list (ValueT.get_idTs vp.(fst)))
       ++ (option_to_list (ValueT.get_idTs vp.(snd))).
+
 End ValueTPair.
+Hint Resolve ValueTPair.eq_dec: EqDecDb.
 
-Module ValueTPairFacts := AltUsualFacts ValueTPair.
-
-(* Module ValueTPair_A := Alt_from_AltUsual ValueTPair_AU. *)
-
-(* TODO: universal construction? *)
-(* Module ValueTPair <: UsualDecidableType. *)
-(*   Definition t := (ValueT.t * ValueT.t)%type. *)
-(*   Definition eq := @eq t. *)
-(*   Definition eq_refl := @refl_equal t. *)
-(*   Definition eq_sym := @sym_eq t. *)
-(*   Definition eq_trans := @trans_eq t. *)
-(*   Definition eq_dec (x y:t): {x = y} + {x <> y}. *)
-(*   Proof. *)
-(*     apply prod_dec; *)
-(*     apply ValueT.eq_dec. *)
-(*   Defined. *)
-
-(*   Definition get_idTs (vp: t): list IdT.t := *)
-(*     (option_to_list (ValueT.get_idTs vp.(fst))) *)
-(*       ++ (option_to_list (ValueT.get_idTs vp.(snd))). *)
-(* End ValueTPair. *)
-(* Hint Resolve ValueTPair.eq_dec: EqDecDb. *)
-Hint Resolve ValueTPairFacts.eq_dec_l: EqDecDb.
-
-(* Module ValueTPairSet <: FSetExtra.WSfun ValueTPair. *)
-(*   Include FSetExtra.Make ValueTPair. *)
-
-(*   Definition clear_idt (idt: IdT.t) (t0: t): t := *)
-(*     filter (fun xy => negb (list_inb IdT.eq_dec (ValueTPair.get_idTs xy) idt)) t0 *)
-(*   . *)
-
-(* End ValueTPairSet. *)
-
-Module ValueTPair_OT := OT_from_AltUsual ValueTPair.
-
-
-
+Module ValueTPair_OT := Backport_Alt ValueTPair.
 Module ValueTPairSet.
-  Include MSetAVLExtra ValueTPair_OT.
+  Include FSetAVLExtra ValueTPair_OT.
 
   Definition clear_idt (idt: IdT.t) (t0: t): t :=
-    filter (fun xy => negb (list_inb IdTFacts.eq_dec_l (ValueTPair.get_idTs xy) idt)) t0
+    filter (fun xy => negb (list_inb IdT.eq_dec (ValueTPair.get_idTs xy) idt)) t0
   .
+
 End ValueTPairSet.
 
-Module ValueTPairSetFacts := MSetFactsExtra ValueTPair_OT ValueTPairSet.
-
-(* Module ValueTPairSetFacts := WFacts_fun2 ValueTPair ValueTPairSet. *)
+Module ValueTPairSetFacts := FSetFactsExtra ValueTPair_OT ValueTPairSet.
 
 Module sz_ValueT := prod sz ValueT.
-(* Module Nat_ValueT := OT_from_AltUsual Nat_ValueT_AU. *)
 
 Module Expr <: AltUsual.
   Inductive t_: Type :=
@@ -599,6 +323,28 @@ Module Expr <: AltUsual.
   .
 
   Definition t := t_.
+  Definition eq_dec (x y:t): {x = y} + {x <> y}.
+  Proof.
+    decide equality;
+      try (apply list_eq_dec);
+      try (apply prod_dec);
+      try (apply IdT.eq_dec);
+      try (apply ValueT.eq_dec);
+      try (apply id_dec);
+      try (apply Tag.eq_dec);
+      try (apply sz_dec);
+      try (apply bop_dec);
+      try (apply fbop_dec);
+      try (apply floating_point_dec);
+      try (apply typ_dec);
+      try (apply const_dec);
+      try (apply inbounds_dec);
+      try (apply truncop_dec);
+      try (apply extop_dec);
+      try (apply castop_dec);
+      try (apply cond_dec);
+      try (apply fcond_dec).
+  Defined.
 
   Definition case_order e : OrdIdx.t :=
     match e with
@@ -800,118 +546,61 @@ Module Expr <: AltUsual.
   .
 
 End Expr.
-
-Module ExprFacts := AltUsualFacts Expr.
-
-Hint Resolve ExprFacts.eq_dec_l: EqDecDb.
+Hint Resolve Expr.eq_dec: EqDecDb.
 Coercion Expr.value: ValueT.t >-> Expr.t_.
 
-Module Expr_OT := OrdersAlt.OT_from_Alt Expr.
-
-Module ExprSet.
-  Include MSetAVLExtra Expr_OT.
-
-  (* Definition clear_idt (idt: IdT.t) (t0: t): t := *)
-  (*   filter (fun xy => negb (list_inb IdTFacts.eq_dec_l (ExprPair.get_idTs xy) idt)) t0 *)
-  (* . *)
-End ExprSet.
-
-Module ExprSetFacts := MSetFactsExtra Expr_OT ExprSet.
-
-(* TODO: universal construction? *)
-(* Module ExprPair <: UsualDecidableType. *)
-(*   Definition t := (Expr.t * Expr.t)%type. *)
-(*   Definition eq := @eq t. *)
-(*   Definition eq_refl := @refl_equal t. *)
-(*   Definition eq_sym := @sym_eq t. *)
-(*   Definition eq_trans := @trans_eq t. *)
-(*   Definition eq_dec (x y:t): {x = y} + {x <> y}. *)
-(*   Proof. *)
-(*     apply prod_dec; *)
-(*       apply Expr.eq_dec. *)
-(*   Defined. *)
-
-(*   Definition get_idTs (ep: t): list IdT.t := *)
-(*     (Expr.get_idTs ep.(fst)) *)
-(*       ++ (Expr.get_idTs ep.(snd)). *)
-(* End ExprPair. *)
+Module Expr_OT := Backport_Alt Expr.
+Module ExprSet := FSetAVLExtra Expr_OT.
 
 Module ExprPair <: AltUsual.
   Include prod Expr Expr.
+  Definition eq_dec (x y:t): {x = y} + {x <> y}.
+  Proof.
+    apply prod_dec;
+      apply Expr.eq_dec.
+  Defined.
 
   Definition get_idTs (ep: t): list IdT.t :=
     (Expr.get_idTs ep.(fst))
       ++ (Expr.get_idTs ep.(snd)).
 End ExprPair.
 
-Module ExprPairFacts := AltUsualFacts ExprPair.
-Hint Resolve ExprPairFacts.eq_dec_l: EqDecDb.
-
-Module ExprPair_OT := OrdersAlt.OT_from_Alt ExprPair.
-
+Module ExprPair_OT := Backport_Alt ExprPair.
 Module ExprPairSet.
-  Include MSetAVLExtra ExprPair_OT.
+  Include FSetAVLExtra ExprPair_OT.
 
   Definition clear_idt (idt: IdT.t) (t0: t): t :=
-    filter (fun xy => negb (list_inb IdTFacts.eq_dec_l (ExprPair.get_idTs xy) idt)) t0
+    filter (fun xy => negb (list_inb IdT.eq_dec (ExprPair.get_idTs xy) idt)) t0
   .
 End ExprPairSet.
 
-Module ExprPairSetFacts := MSetFactsExtra ExprPair_OT ExprPairSet.
-
-
-(* Module ExprPairSet <: FSetExtra.WSfun ExprPair. *)
-(*   Include FSetExtra.Make ExprPair. *)
-
-(*   Definition clear_idt (idt: IdT.t) (t0: t): t := *)
-(*     filter (fun xy => negb (list_inb IdT.eq_dec (ExprPair.get_idTs xy) idt)) t0 *)
-(*   . *)
-
-(* End ExprPairSet. *)
-
-(* Module ExprPairSetFacts := WFacts_fun2 ExprPair ExprPairSet. *)
+Module ExprPairSetFacts := FSetFactsExtra ExprPair_OT ExprPairSet.
 
 (* Ptr: alias related values *)
-(* Module Ptr <: UsualDecidableType. *)
-(*   (* typ has the type of the 'pointer', not the type of the 'object'. *)
-(*      ex: %x = load i32* %y, align 4 <- (id y, typ_pointer (typ_int 32)) *)
-(*                    ^^^^ *)
-(*   *) *)
-(*   Definition t := (ValueT.t * typ)%type. *)
-(*   Definition eq := @eq t. *)
-(*   Definition eq_refl := @refl_equal t. *)
-(*   Definition eq_sym := @sym_eq t. *)
-(*   Definition eq_trans := @trans_eq t. *)
-(*   Definition eq_dec (x y:t): {x = y} + {x <> y}. *)
-(*   Proof. *)
-(*     apply prod_dec. *)
-(*     apply ValueT.eq_dec. *)
-(*     apply typ_dec. *)
-(*   Defined. *)
-(*   Definition get_idTs (p: t): option IdT.t := *)
-(*     match p with *)
-(*     | (v,_) => ValueT.get_idTs v *)
-(*     end. *)
-(* End Ptr. *)
-
 Module Ptr <: AltUsual.
+  (* typ has the type of the 'pointer', not the type of the 'object'.
+     ex: %x = load i32* %y, align 4 <- (id y, typ_pointer (typ_int 32))
+                   ^^^^
+  *)
   Include prod ValueT typ.
+
+  Definition eq_dec (x y:t): {x = y} + {x <> y}.
+  Proof.
+    apply prod_dec.
+    apply ValueT.eq_dec.
+    apply typ_dec.
+  Defined.
 
   Definition get_idTs (p: t): option IdT.t :=
     match p with
     | (v,_) => ValueT.get_idTs v
     end.
+
 End Ptr.
 
-Module PtrFacts := AltUsualFacts Ptr.
-
-Module Ptr_OT := OrdersAlt.OT_from_Alt Ptr.
-
-Module PtrSet := MSetAVLExtra Ptr_OT.
-Module PtrSetFacts := MSetFactsExtra Ptr_OT PtrSet.
-
-(* Module PtrSet : FSetExtra.WSfun Ptr := FSetExtra.Make Ptr. *)
-(* Module PtrSetFacts := WFacts_fun2 Ptr PtrSet. *)
+Module Ptr_OT := Backport_Alt Ptr.
+Module PtrSet := FSetAVLExtra Ptr_OT.
+Module PtrSetFacts := FSetFactsExtra Ptr_OT PtrSet.
 
 Lemma InA_equiv_eqs
       X (eqa eqb : X -> X -> Prop)
@@ -934,53 +623,44 @@ Proof.
   apply InA_equiv_eqs.
   i. split.
   - apply Ptr.compare_leibniz.
-  - i. subst. apply PtrFacts.compare_refl.
+  - i. subst. apply PtrSet.E.eq_refl.
 Qed.
 
 Module PtrPair <: AltUsual.
   Include prod Ptr Ptr.
+  Definition eq_dec (x y:t): {x = y} + {x <> y}.
+  Proof.
+    apply prod_dec; apply Ptr.eq_dec.
+  Defined.
 
   Definition get_idTs (pp: t): list IdT.t :=
     (option_to_list (Ptr.get_idTs pp.(fst)))
       ++ (option_to_list (Ptr.get_idTs pp.(snd))).
 End PtrPair.
+Hint Resolve PtrPair.eq_dec: EqDecDb.
 
-(* Module PtrPair <: UsualDecidableType. *)
-(*   Definition t := (Ptr.t * Ptr.t)%type. *)
-(*   Definition eq := @eq t. *)
-(*   Definition eq_refl := @refl_equal t. *)
-(*   Definition eq_sym := @sym_eq t. *)
-(*   Definition eq_trans := @trans_eq t. *)
-(*   Definition eq_dec (x y:t): {x = y} + {x <> y}. *)
-(*   Proof. *)
-(*     apply prod_dec; apply Ptr.eq_dec. *)
-(*   Defined. *)
-
-(*   Definition get_idTs (pp: t): list IdT.t := *)
-(*     (option_to_list (Ptr.get_idTs pp.(fst))) *)
-(*       ++ (option_to_list (Ptr.get_idTs pp.(snd))). *)
-(* End PtrPair. *)
-Module PtrPairFacts := AltUsualFacts PtrPair.
-Hint Resolve PtrPairFacts.eq_dec_l: EqDecDb.
-
-(* Module PtrPairSet <: FSetExtra.WSfun PtrPair. *)
-(*   Include FSetExtra.Make PtrPair. *)
-
-(*   Definition clear_idt (idt: IdT.t) (t0: t): t := *)
-(*     filter (fun xy => negb (list_inb IdT.eq_dec (PtrPair.get_idTs xy) idt)) t0 *)
-(*   . *)
-
-(* End PtrPairSet. *)
-(* Module PtrPairSetFacts := WFacts_fun2 PtrPair PtrPairSet. *)
-
-Module PtrPair_OT := OrdersAlt.OT_from_Alt PtrPair.
+Module PtrPair_OT := Backport_Alt PtrPair.
 
 Module PtrPairSet.
-  Include MSetAVLExtra PtrPair_OT.
+  Include FSetAVLExtra PtrPair_OT.
   Definition clear_idt (idt: IdT.t) (t0: t): t :=
-    filter (fun xy => negb (list_inb IdTFacts.eq_dec_l (PtrPair.get_idTs xy) idt)) t0
+    filter (fun xy => negb (list_inb IdT.eq_dec (PtrPair.get_idTs xy) idt)) t0
   .
 
 End PtrPairSet.
 
-Module PtrPairSetFacts := MSetFactsExtra PtrPair_OT PtrPairSet.
+Module PtrPairSetFacts := FSetFactsExtra PtrPair_OT PtrPairSet.
+
+
+
+(* TODO: Remove this after migrating yoonseung's Ords.v *)
+Ltac solve_leibniz_ cmp CL :=
+  repeat match goal with
+         | [H:cmp ?a ?b = Eq |- _] => apply CL in H
+         end; subst.
+
+Ltac solve_leibniz :=
+  solve_leibniz_ ExprPair.compare ExprPair.compare_leibniz;
+  solve_leibniz_ ValueTPair.compare ValueTPair.compare_leibniz;
+  solve_leibniz_ PtrPair.compare PtrPair.compare_leibniz
+.
